A branch that reproves properties about FV and CoreFVs using StrongSubset

examples/ghc/theories/ScopeInvariant.v
@@ -22,35 +22,16 @@ Require Import Proofs.Base.
 Require Import Proofs.GhcTactics.
 Require Import Proofs.Forall.
 Require Import Proofs.Unique.
-Require Import Proofs.CoreFVs. 
+Require Import Proofs.Var.
 Require Import Proofs.VarSet.
-Require Import Proofs.VarSetStrong.
 Require Import Proofs.VarEnv.
 Require Import Proofs.CoreInduct.
-Require Import Proofs.Var.
+
 
 Import GHC.Base.Notations.
 
 Set Bullet Behavior "Strict Subproofs".
 Opaque GHC.Base.hs_string__.
-
-Lemma contrapositive : forall (A B:Prop), (A -> B) -> (~ B) -> (~ A).
-Proof.
-  intros.
-  intro h. apply H in h. apply H0. auto.
-Qed.
-
-Lemma and_iff_compat_both:
-  forall A B C D : Prop,
-    A <-> C -> B <-> D ->
-    A /\ B <-> C /\ D.
-Proof. intros. intuition. Qed.
-
-Lemma Forall_iff:
-  forall a P Q (xs : list a),
-    Forall (fun x => P x <-> Q x) xs ->
-    Forall P xs <-> Forall Q xs.
-Proof. intros. rewrite -> !Forall_forall in *. firstorder. Qed.
 
 
 (** * Core invariants related to variables and scope *)
@@ -87,9 +68,6 @@ Definition GoodVar (v : Var) : Prop :=
 Definition GoodLocalVar (v : Var) : Prop :=
   GoodVar v /\ isLocalVar v = true.
 
-
-
-
 (**
 
 Next we define when a variable occurrence is ok in a given scope.
@@ -101,12 +79,11 @@ Next we define when a variable occurrence is ok in a given scope.
 *)
 
 Definition WellScopedVar (v : Var) (in_scope : VarSet) : Prop :=
-  if isLocalVar v then
    match lookupVarSet in_scope v with
     | None => False
     | Some v' => almostEqual v v' /\ GoodVar v
-    end
-  else GoodVar v (* we do not track global variables yet *).
+    end.
+
 
 (**
 
@@ -253,9 +230,7 @@ Proof.
   intros.
   unfold WellScopedVar.
   rewrite lookupVarSet_extendVarSet_self.
-  destruct_match.
-  * split. apply almostEqual_refl. trivial.
-  * trivial.
+  split. apply almostEqual_refl. trivial.
 Qed.
 
 Lemma WellScoped_varToCoreExpr:
@@ -335,198 +310,6 @@ Proof.
   split; intro; repeat split; try constructor; intuition.
 Qed.
 
-(** *** Lemmas related to [StrongSubset] *)
-
-Lemma WellScopedVar_StrongSubset : forall e vs1 vs2, 
-    WellScopedVar e vs1 -> StrongSubset vs1 vs2 -> WellScopedVar e vs2.
-Proof.
-  intros v vs1 vs2 WS SS.
-  unfold WellScopedVar, StrongSubset in *.
-  destruct_match; only 2: trivial.
-  specialize (SS v).
-  destruct (lookupVarSet vs1 v); try contradiction.
-  destruct (lookupVarSet vs2 v) eqn:LV2; try contradiction.
-  intuition.
-  eapply almostEqual_trans with (v2 := v0); auto.
-Qed.
-
-
-(* No such thing as WellScopedTickish anymore *)
-(*
-Lemma WellScopedTickish_StrongSubset : forall e vs1 vs2, 
-    WellScopedTickish e vs1 -> StrongSubset vs1 vs2 -> WellScopedTickish e vs2.
-Proof.
-  move => e vs1 vs2 WS SS.
-  unfold WellScopedTickish, StrongSubset in *.
-  destruct_match; try done.
-  eapply Forall_impl; eauto.
-  move=> a h. eapply WellScopedVar_StrongSubset; eauto. simpl in h.
-  auto.
-Qed.
-*)
-
-Lemma WellScoped_StrongSubset : forall e vs1 vs2, 
-    WellScoped e vs1 -> StrongSubset vs1 vs2 -> WellScoped e vs2.
-Proof.
-  intro e.
-  apply (core_induct e); intros; try (destruct binds);
-    unfold WellScoped in *; fold WellScoped in *; eauto.
-  - eapply WellScopedVar_StrongSubset; eauto.
-  - destruct H1. split; eauto.
-  - split; only 1: apply H0.
-    destruct H0 as [_ H0].
-    eapply H; eauto.
-    unfold StrongSubset in *.
-    intro var.
-    specialize (H1 var).
-    unfold CoreBndr in v. (* make sure that the type class looks right.*)
-    destruct (v GHC.Base.== var) eqn:Eq.
-    + rewrite lookupVarSet_extendVarSet_eq; auto.
-      rewrite lookupVarSet_extendVarSet_eq; auto.
-      eapply almostEqual_refl.
-    + rewrite lookupVarSet_extendVarSet_neq.
-      destruct (lookupVarSet vs1 var) eqn:IN; auto.
-      rewrite lookupVarSet_extendVarSet_neq.
-      auto.
-      intro h;
-      rewrite Eq in h; discriminate.
-      intro h;
-      rewrite Eq in h; discriminate.
-  - destruct H1 as [[GLV WE] Wb].
-     split; only 1: split; eauto.
-     eapply H0; eauto.
-     eapply StrongSubset_extendVarSetList.
-     auto.
-  - destruct H1 as [[WE1 [WE2 WE3]] Wb].
-     repeat split; auto.
-     rewrite -> Forall'_Forall in *.
-     rewrite -> Forall_forall in *.
-     intros h IN. destruct h as [v rhs].
-     specialize (WE3 (v,rhs)).
-     simpl in *.
-     eauto using StrongSubset_extendVarSetList.
-     eauto using StrongSubset_extendVarSetList.
-  - destruct H1 as [W1 [W2 W3]].    split; only 2: split; eauto.
-     rewrite -> Forall'_Forall in *.
-     rewrite -> Forall_forall in *.
-     intros h IN. destruct h as [[dc pats] rhs].
-     specialize (H0 dc pats rhs IN).
-     specialize (W3 (dc,pats,rhs) IN).
-     simpl in *.
-     destruct W3 as [GLV WS].
-     eauto using StrongSubset_extendVarSetList.
-(*
-  - move: H0 => [? ?].
-    eauto using WellScopedTickish_StrongSubset.
-*)
-Qed.
-
-(** *** Relation to [exprFreeVars] *)
-
-Require Import Proofs.VarSetFSet.
-
-Lemma WellScoped_subset:
-  forall e vs,
-    WellScoped e vs -> subVarSet (exprFreeVars e) vs = true.
-Proof.
-  intro e.
-  apply (core_induct e); intros.
-  - unfold WellScoped, WellScopedVar in *.
-    destruct (isLocalVar v) eqn:HisLocal.
-    + destruct (lookupVarSet vs v) eqn:Hl; try contradiction.
-      rewrite -> exprFreeVars_Var by assumption.
-      rewrite subVarSet_unitVarSet.
-      eapply lookupVarSet_elemVarSet; eassumption.
-    + rewrite -> exprFreeVars_global_Var by assumption.
-      apply subVarSet_emptyVarSet. 
-  - apply subVarSet_emptyVarSet.
-  - simpl in H1.
-    rewrite exprFreeVars_App.
-    rewrite subVarSet_unionVarSet.
-    rewrite andb_true_iff.
-    intuition.
-  - simpl in H0.
-    destruct H0.
-    rewrite exprFreeVars_Lam.
-    apply H in H1.
-    set_b_iff. fsetdec.
-  - destruct binds as [v rhs | pairs].
-    + simpl in H1. decompose [and] H1; clear H1.
-      rewrite exprFreeVars_Let_NonRec.
-      apply H in H5.
-      apply H0 in H3.
-      rewrite -> extendVarSetList_cons, extendVarSetList_nil in H3.
-      set_b_iff. fsetdec.
-    + simpl in H1. decompose [and] H1; clear H1.
-      rewrite -> Forall'_Forall in H6.
-      rewrite exprFreeVars_Let_Rec.
-      apply H0 in H3; clear H0.
-      rewrite Core.bindersOf_Rec_cleanup in H3.
-      apply subVarSet_delVarSetList_extendVarSetList_dual.
-      unfold is_true.
-      rewrite -> subVarSet_unionVarSet, andb_true_iff; split.
-      * apply subVarSet_exprsFreeVars.
-        rewrite -> Forall_map, Forall_forall in *.
-        intros [v rhs] HIn. simpl in *.
-        apply (H _ _ HIn).
-        apply (H6 _ HIn).
-      * assumption.
-  - simpl in H1. decompose [and] H1; clear H1.
-    rewrite -> Forall'_Forall in H5.
-    rewrite exprFreeVars_Case.
-    rewrite -> subVarSet_unionVarSet, andb_true_iff; split.
-    * apply H; assumption.
-    * apply subVarSet_mapUnionVarSet.
-      rewrite -> Forall_forall in *.
-      intros [[dc pats] rhs] HIn.
-      specialize (H5 _ HIn). destruct H5. simpl in *.
-      (* Some reordering is needed here. This is a bit smelly,
-         maybe there should be a [rev] in [exprFreeVars_Case] already? *)
-      rewrite <- delVarSetList_rev.
-      rewrite rev_app_distr.
-      rewrite delVarSetList_app.
-      rewrite !delVarSetList_rev.
-      rewrite <- delVarSetList_app.
-      simpl.
-      apply subVarSet_delVarSetList_extendVarSetList_dual.
-      apply (H0 _ _ _ HIn).
-      assumption.
-  - rewrite exprFreeVars_Cast. apply H; assumption.
-(*  - rewrite exprFreeVars_Tick.
-    simpl in H0.
-    by apply H.
-
-    rewrite exprFreeVars_Tick. 
-    simpl in H0. move: H0 => [a b].
-    destruct tickish; unfold tickishFreeVars in *; hs_simpl;
-      try (apply H; assumption).
-    simpl in b.
-    rewrite -> subVarSet_unionVarSet, andb_true_iff; split.
-    eauto.
-    set_b_iff.
-    move=> x InX.
-    rewrite -> filter_iff in InX; try apply RespectsVar_isLocalVar.
-    move: InX => [i0 i1].
-    rewrite -> Forall_forall in b.
-    rewrite -> extendVarSetList_iff in i0.
-    destruct i0; try done.
-    unfold In.
-    move: (elem_exists_in _ _ H0) => [y [Iny eqy]].
-    move: (b _ Iny) => WSy.
-    unfold WellScopedVar in WSy.
-
-    rewrite (RespectsVar_isLocalVar eqy) in i1.
-    rewrite i1 in WSy.
-    elim h: (lookupVarSet vs y) => [z|].
-    erewrite (elemVarSet_eq _ eqy); eauto.
-    eapply lookupVarSet_elemVarSet; eauto.
-    rewrite h in WSy. done.
-    *)
-  - apply subVarSet_emptyVarSet.
-  - apply subVarSet_emptyVarSet. 
-Qed.
-
-
 (** *** Freshness *)
 
 Lemma WellScopedVar_extendVarSetList_l:
@@ -537,10 +320,9 @@ Lemma WellScopedVar_extendVarSetList_l:
 Proof.
   intros.
   unfold WellScopedVar in *.
-  destruct_match; only 2: assumption.
   destruct_match; only 2: contradiction.
   rewrite lookupVarSet_extendVarSetList_l. 
-  rewrite Heq0.
+  rewrite Heq.
   assumption.
   rewrite H0. 
   auto.
@@ -557,437 +339,12 @@ Proof.
   unfold WellScopedVar in *.
   assert (Gv: GoodVar v). 
    { rewrite -> Forall_forall in *. auto. }
-  destruct_match.
-  rewrite -> lookupVarSet_extendVarSetList_self_in by assumption.
+  rewrite -> lookupVarSet_extendVarSetList_self_in by assumption. 
   intuition.
-  assumption.
 Qed.
 
-
-Lemma WellScopedVar_extendVarSetList_fresh_under v vs vs1 vs2 :
-  disjointVarSet (delVarSetList (exprFreeVars (Mk_Var v)) (rev vs2))
-                 (mkVarSet vs1) = true ->
-  WellScopedVar v (extendVarSetList (extendVarSetList vs vs1) vs2) <->
-  WellScopedVar v (extendVarSetList vs vs2).
-Proof.
-    intro H.
-    unfold WellScopedVar.
-    destruct_match; only 2: reflexivity.
-    enough (lookupVarSet (extendVarSetList (extendVarSetList vs vs1) vs2) v = 
-            lookupVarSet (extendVarSetList vs vs2) v) as Htmp
-      by (rewrite Htmp; reflexivity).
-    rewrite -> exprFreeVars_Var in H by assumption.
-    setoid_rewrite delVarSetList_rev in H.
-    clear -H.
-    (* duplication with isJoinPointsValid_fresh_updJPSs_aux here *)
-    induction vs2 using rev_ind.
-    + rewrite !extendVarSetList_nil.
-      rewrite delVarSetList_nil in H.
-      revert vs; induction vs1; intros.
-      - rewrite extendVarSetList_nil.
-        reflexivity.
-      - rewrite extendVarSetList_cons.
-        rewrite -> fold_is_true in H.
-        rewrite -> disjointVarSet_mkVarSet_cons in H.
-        destruct H.
-        rewrite -> IHvs1 by assumption.
-        apply lookupVarSet_extendVarSet_neq.
-        rewrite <- elemVarSet_unitVarSet_is_eq. intro.
-        contradict H. rewrite H1=>//.
-    + rewrite -> delVarSetList_app, delVarSetList_cons, delVarSetList_nil in H.
-      rewrite -> !extendVarSetList_append, !extendVarSetList_cons, !extendVarSetList_nil.
-      destruct (x GHC.Base.== v) eqn:?.
-      -- rewrite -> !lookupVarSet_extendVarSet_eq by assumption.
-         reflexivity.
-      -- rewrite <- not_true_iff_false in Heqb.
-         rewrite -> !lookupVarSet_extendVarSet_neq by assumption.
-         apply IHvs2.
-         rewrite -> fold_is_true in *.
-         rewrite -> disjointVarSet_mkVarSet in *.
-         eapply Forall_impl; only 2: eapply H. intros v2 ?.
-         cbv beta in H0.
-         rewrite -> delVarSet_elemVarSet_false in H0; only 1: assumption.
-         clear -Heqb.
-         apply elemVarSet_delVarSetList_false_l.
-         rewrite elemVarSet_unitVarSet_is_eq.
-         apply negbTE, notE => //. 
-Qed.
-
-
-(* There are a number of variants of the freshness lemmas.
-   The simplest one that implies all others is this, so lets
-   only do one induction:
-*)
-
-
-
-Lemma WellScoped_extendVarSetList_fresh_under:
-  forall vs1 vs2 e vs,
-  disjointVarSet (delVarSetList (exprFreeVars e) vs2) (mkVarSet vs1)  = true ->
-  WellScoped e (extendVarSetList (extendVarSetList vs vs1) vs2) <->
-  WellScoped e (extendVarSetList vs vs2).
-Proof.
- (* This proof is similar to isJoinPointsValid_fresh_updJPSs_aux
-    In particular, proving the assumtion [disjointVarSet ..] for all the inductive
-    cases is identical (although here we have more inductive cases than there.
-    Once could common it up with a deidcated induction rule. Or live with the duplication.
-  *)
-  intros.
-  rewrite <- delVarSetList_rev in H.
-  revert vs2 vs H.
-  apply (core_induct e); intros.
-  * simpl.
-    eapply WellScopedVar_extendVarSetList_fresh_under; eauto.
-  * reflexivity.
-  * simpl.
-    apply and_iff_compat_both.
-    - apply H.
-      eapply disjointVarSet_subVarSet_l; only 1: apply H1.
-      apply subVarSet_delVarSetList_both.
-      rewrite exprFreeVars_App.
-      set_b_iff; fsetdec.
-    - apply H0.
-      eapply disjointVarSet_subVarSet_l; only 1: apply H1.
-      apply subVarSet_delVarSetList_both.
-      rewrite exprFreeVars_App.
-      set_b_iff; fsetdec.
-  * simpl.
-    apply and_iff_compat_both; try reflexivity.
-    rewrite <- !extendVarSetList_singleton.
-    rewrite <- !extendVarSetList_append with (vs1 := vs2).
-    apply H.
-    rewrite -> exprFreeVars_Lam in H0.
-    rewrite rev_app_distr.
-    simpl.
-    rewrite delVarSetList_cons.
-    assumption.
-  * simpl.
-    apply and_iff_compat_both.
-    - destruct binds as [v rhs | pairs].
-      + simpl.
-        apply and_iff_compat_both; only 1: reflexivity.
-        apply H.
-        eapply disjointVarSet_subVarSet_l; only 1: apply H1.
-        apply subVarSet_delVarSetList_both.
-        rewrite exprFreeVars_Let_NonRec.
-        set_b_iff; fsetdec.
-      + simpl.
-        repeat apply and_iff_compat_both; try reflexivity.
-        rewrite !Forall'_Forall.
-        apply Forall_iff.
-        rewrite Forall_forall.
-        intros [v rhs] HIn.
-        rewrite <- !extendVarSetList_append with (vs1 := vs2).
-        apply (H _ _ HIn).
-        eapply disjointVarSet_subVarSet_l; only 1: apply H1.
-        rewrite rev_app_distr; simpl.
-        rewrite delVarSetList_app.
-        apply subVarSet_delVarSetList_both.
-        rewrite exprFreeVars_Let_Rec.
-        pose proof (subVarSet_exprFreeVars_exprsFreeVars _ _ _ HIn).
-        rewrite delVarSetList_rev.
-        apply subVarSet_delVarSetList_both.
-        set_b_iff; fsetdec.
-    - rewrite <- !extendVarSetList_append with (vs1 := vs2).
-      apply H0.
-      eapply disjointVarSet_subVarSet_l; only 1: apply H1; clear H1.
-      rewrite -> rev_app_distr, delVarSetList_app.
-      apply subVarSet_delVarSetList_both.
-      destruct binds as [v rhs | pairs].
-      -- rewrite exprFreeVars_Let_NonRec.
-         simpl.
-         rewrite -> delVarSetList_cons, delVarSetList_nil.
-         set_b_iff; fsetdec.
-      -- rewrite exprFreeVars_Let_Rec.
-         simpl. rewrite Core.bindersOf_Rec_cleanup.
-         rewrite delVarSetList_rev.
-         apply subVarSet_delVarSetList_both.
-         set_b_iff; fsetdec.
-
-  * simpl.
-    repeat apply and_iff_compat_both; try reflexivity.
-    - apply H.
-      eapply disjointVarSet_subVarSet_l; only 1: apply H1; clear H1.
-      apply subVarSet_delVarSetList_both.
-      rewrite exprFreeVars_Case.
-      set_b_iff; fsetdec.
-    - rewrite !Forall'_Forall.
-      apply Forall_iff.
-      rewrite Forall_forall.
-      intros [[dc pats] rhs] HIn; simpl.
-      repeat apply and_iff_compat_both; try reflexivity.
-      rewrite <- !extendVarSetList_append with (vs1 := vs2).
-      apply (H0 _ _ _ HIn).
-      eapply disjointVarSet_subVarSet_l; only 1: apply H1.
-      rewrite rev_app_distr; simpl.
-      rewrite -> !delVarSetList_app, delVarSetList_cons, delVarSetList_nil.
-      apply subVarSet_delVarSetList_both.
-      rewrite exprFreeVars_Case.
-      unfold is_true.
-      match goal with HIn : List.In _ ?xs |- context [mapUnionVarSet ?f ?xs] =>
-        let H := fresh in
-        epose proof (mapUnionVarSet_In_subVarSet f HIn) as H ; simpl in H end.
-      rewrite -> delVarSetList_rev, <- delVarSetList_single, <- delVarSetList_app.
-      set_b_iff; fsetdec.
-  * apply H. 
-    eapply disjointVarSet_subVarSet_l; only 1: apply H0.
-    apply subVarSet_delVarSetList_both.
-    rewrite exprFreeVars_Cast.
-    set_b_iff; fsetdec.
-(*  * simpl.
-    apply H.
-    eapply disjointVarSet_subVarSet_l; only 1: apply H0.
-    apply subVarSet_delVarSetList_both.
-    rewrite exprFreeVars_Tick.
-    set_b_iff; fsetdec.
-    (*
-    simpl.
-    eapply and_iff_compat_both.
-    ++ apply H.
-       eapply disjointVarSet_subVarSet_l; only 1: apply H0.
-       apply subVarSet_delVarSetList_both.
-       rewrite exprFreeVars_Tick.
-       set_b_iff; fsetdec. 
-    ++ destruct tickish; try done.
-       simpl. 
-       rewrite -> exprFreeVars_Tick in H0.
-       apply Forall_iff.
-       rewrite Forall_forall.
-       move=> x In.
-       eapply WellScopedVar_extendVarSetList_fresh_under.
-       unfold tickishFreeVars in H0.
-       eapply disjointVarSet_subVarSet_l.
-       eapply H0.
-       eapply subVarSet_delVarSetList_both.
-       elim LV: (isLocalVar x).
-       -- rewrite (exprFreeVars_Var x LV).
-          rewrite subVarSet_unitVarSet.
-          hs_simpl. apply /orP. right.
-          rewrite elemVarSet_filterVarSet => //.
-          apply /andP. split. auto.
-          hs_simpl.
-          apply list_in_elem.
-          auto.
-       -- rewrite (exprFreeVars_global_Var x LV).
-          apply subVarSet_emptyVarSet.
-    *) *)
-  * reflexivity.
-  * reflexivity. 
-Qed.
-
-Lemma WellScoped_extendVarSetList_fresh:
-  forall vs e vs1,
-  disjointVarSet (exprFreeVars e) (mkVarSet vs) = true ->
-  WellScoped e (extendVarSetList vs1 vs) <->
-  WellScoped e vs1.
-Proof.
-  intros.
-  epose proof (WellScoped_extendVarSetList_fresh_under vs [] e vs1 _).
-  rewrite !extendVarSetList_nil in H0.
-  eassumption.
-  Unshelve.
-  rewrite delVarSetList_nil. assumption.
-Qed.
-
-Lemma WellScoped_extendVarSet_fresh:
-  forall v e vs,
-  elemVarSet v (exprFreeVars e) = false ->
-  WellScoped e (extendVarSet vs v) <-> WellScoped e vs.
-Proof.
-  intros.
-  epose proof (WellScoped_extendVarSetList_fresh [v] e vs _).
-  rewrite -> extendVarSetList_cons,extendVarSetList_nil in H0.
-  assumption.
-  Unshelve.
-  rewrite -> fold_is_true in *.
-  rewrite -> disjointVarSet_mkVarSet_cons, disjointVarSet_mkVarSet_nil.
-  intuition congruence.
-Qed.
-
-Lemma WellScoped_extendVarSetList_fresh_between:
-  forall (vs1 vs2 vs3 : list Var) (e : CoreExpr) (vs : VarSet),
-  disjointVarSet (delVarSetList (exprFreeVars e) vs3) (mkVarSet vs2) = true ->
-  WellScoped e (extendVarSetList vs ((vs1 ++ vs2) ++ vs3)) <->
-  WellScoped e (extendVarSetList vs (vs1 ++ vs3)).
-Proof.
-  intros.
-  rewrite <- app_assoc.
-  rewrite !extendVarSetList_append.
-  apply WellScoped_extendVarSetList_fresh_under.
-  assumption.
-Qed.
 
 (** *** The invariants respect [StrongSubset] *)
 
 
-Instance Respects_StrongSubset_WellScopedVar v : Respects_StrongSubset (WellScopedVar v).
-Proof.
-  intros ????.
-  unfold WellScopedVar in *.
-  destruct_match; only 2: assumption.
-  destruct_match; only 2: contradiction.
-  specialize (H v).
-  rewrite Heq0 in H.
-  destruct_match; only 2: contradiction.
-  intuition.
-  eapply almostEqual_trans; eassumption.
-Qed.
 
-(*
-Instance Respects_StrongSubset_WellScopedTickish v : Respects_StrongSubset (WellScopedTickish v).
-Proof.
-  intros ????.
-  unfold WellScopedTickish in *.
-  destruct v; try done.
-  rewrite -> Forall_forall in *.
-  move=> x In.
-  move: (H0 x In) => h.
-  eapply Respects_StrongSubset_WellScopedVar; eauto.
-Qed.
-*)
-
-Instance Respects_StrongSubset_WellScoped e : Respects_StrongSubset (WellScoped e).
-Proof.
-  apply (core_induct e); intros; simpl.
-  * apply Respects_StrongSubset_WellScopedVar.
-  * apply Respects_StrongSubset_const.
-  * apply Respects_StrongSubset_and; assumption.
-  * apply Respects_StrongSubset_and; try apply Respects_StrongSubset_const.
-    apply Respects_StrongSubset_extendVarSet.
-    assumption.
-  * apply Respects_StrongSubset_and.
-    - destruct_match.
-      + apply Respects_StrongSubset_and; try apply Respects_StrongSubset_const.
-        assumption.
-      + simpl.
-        repeat apply Respects_StrongSubset_and; try apply Respects_StrongSubset_const.
-        setoid_rewrite Forall'_Forall.
-        apply Respects_StrongSubset_forall.
-        rewrite Forall_forall.
-        intros [v rhs] HIn.
-        specialize (H _ _ HIn).
-        apply Respects_StrongSubset_extendVarSetList.
-        apply H.
-    - apply Respects_StrongSubset_extendVarSetList.
-      apply H0.
-   * repeat apply Respects_StrongSubset_and; try apply Respects_StrongSubset_const.
-     - apply H.
-     - setoid_rewrite Forall'_Forall.
-       apply Respects_StrongSubset_forall.
-       rewrite Forall_forall.
-       intros [[dc pats] rhs] HIn.
-       repeat apply Respects_StrongSubset_and; try apply Respects_StrongSubset_const.
-       specialize (H0 _ _ _ HIn).
-       apply Respects_StrongSubset_extendVarSetList.
-       apply H0.
-   * apply H.
-(*   * apply H.
-     (*
-     unfold Respects_StrongSubset
-     move=> vs1 vs2 SS.
-     move=> [WSE WST].
-     split.
-     eauto.
-     eapply Respects_StrongSubset_WellScopedTickish; eauto.
-     *) *)
-   * apply Respects_StrongSubset_const.
-   * apply Respects_StrongSubset_const. 
-Qed.
-
-
-
-(* This seems straitforward to prove given our current
-   theories of exprFreeVars. 
-   However, a stronger result is possible: that the free vars  
-   are a *strong subset* of the in_scope set.
-*)
-Lemma WellScoped_exprFreeVars :
-  forall e vs, WellScoped e vs -> exprFreeVars e [<=] vs.
-Proof.
-  intro e. apply (core_induct e); intros; unfold WellScoped in H.
-  - destruct (isLocalVar v) eqn:L.
-    + rewrite exprFreeVars_Var; auto.
-      unfold WellScopedVar in H. rewrite L in H.
-      destruct (lookupVarSet vs v) eqn: K; try done.
-      move: (lookupVarSet_elemVarSet K) => K2.
-      set_b_iff.
-      rewrite singleton_equal_add.
-      eapply subset_add_3; auto.
-      fsetdec.
-    + rewrite exprFreeVars_global_Var; auto.
-      fsetdec.
-  - hs_simpl. fsetdec.
-  - fold WellScoped in H. simpl in H1.
-    move: H1 => [he1 he2]. 
-    rewrite exprFreeVars_App.
-    rewrite H; eauto. rewrite H0; eauto. fsetdec.
-  - fold WellScoped in H. simpl in H0.
-    move: H0 => [GV WS].
-    rewrite exprFreeVars_Lam.
-    apply H in WS. 
-    set_b_iff.
-    rewrite WS.
-    fsetdec.
-  - fold WellScoped in H. simpl in H1.
-    move: H1 => [WSbi WSbo].
-    destruct binds; simpl in WSbi.
-    + rewrite exprFreeVars_Let_NonRec.
-      move: WSbi => [Gc WSe0].
-      apply H in WSe0.
-      apply H0 in WSbo.
-      simpl in WSbo.
-      autorewrite with hs_simpl in WSbo.
-      eapply union_subset_3; auto.
-      set_b_iff.
-      fsetdec.
-    + rewrite exprFreeVars_Let_Rec.
-      move: WSbi => [Gc[ nd FWSe0]].
-      apply H0 in WSbo. 
-      unfold bindersOf in WSbo.
-      rewrite Core.bindersOf_Rec_cleanup in WSbo.
-      rewrite <- SubsetE.
-      apply subVarSet_delVarSetList_extendVarSetList_dual.
-      unfold is_true.
-      rewrite -> subVarSet_unionVarSet, andb_true_iff; split.
-      * apply subVarSet_exprsFreeVars.
-        rewrite -> Forall_map, Forall_forall in *.
-        intros [v rhs] HIn. simpl in *.
-        specialize (H _ _ HIn (extendVarSetList vs (map fst l))).
-        rewrite <- SubsetE in H. eapply H.
-        rewrite -> Forall'_Forall in FWSe0.
-        rewrite -> Forall_forall in FWSe0.
-        apply (FWSe0 _ HIn).
-      * rewrite <- SubsetE in WSbo.
-        auto.
-  - fold WellScoped in H. simpl in H1.
-    move: H1 => [WSs [GVb FF]].
-    rewrite exprFreeVars_Case.
-    apply H in WSs.
-    eapply union_subset_3; auto.
-    rewrite -> Forall'_Forall in FF. rewrite -> Forall_forall in FF.
-    rewrite <- SubsetE.
-    eapply subVarSet_mapUnionVarSet.
-    rewrite -> Forall_forall.
-    move=> x In.
-    move: (FF x In) => [h0 h1].
-    destruct x as [[dc pats] rhs].
-    specialize (H0 dc pats rhs In).
-    rewrite <- delVarSetList_rev.
-    (* smelly reverse *)
-    rewrite rev_app_distr.
-    rewrite delVarSetList_app.
-    rewrite !delVarSetList_rev.
-    rewrite <- delVarSetList_app.
-
-    eapply subVarSet_delVarSetList_extendVarSetList_dual.
-    rewrite -> SubsetE.
-    eapply H0.
-    eapply h1.
-  - fold WellScoped in H. simpl in H0.
-    rewrite exprFreeVars_Cast.
-    eauto.
-  - rewrite exprFreeVars_Type.
-    fsetdec.
-  - rewrite exprFreeVars_Coercion.
-    fsetdec.
-Qed.
