examples/ghc/theories/CoreTidy.v
@@ -1,0 +1,68 @@
+(* Disable notation conflict warnings *)
+Set Warnings "-notation-overridden".
+
+
+From mathcomp.ssreflect
+Require Import ssreflect ssrnat prime ssrbool eqtype.
+
+
+Require Import GHC.Base.
+Require Import CoreFVs.
+Require Import Id.
+Require Import Core.
+Require Import CoreTidy.
+
+Require Import Proofs.Prelude.
+
+Require Import Coq.Lists.List.
+Import ListNotations.
+Require Import Coq.NArith.BinNat.
+Require Import Coq.Program.Equality. (* for dependent destruction *)
+ 
+Require Import Coq.Logic.FunctionalExtensionality.
+
+Require Import Proofs.Axioms.
+Require Import Proofs.Base.
+Require Import Proofs.ScopeInvariant.
+Require Import Proofs.CoreInduct.
+Require Import Proofs.Core.
+Require Import Proofs.CoreFVs.
+Require Import Proofs.GhcTactics.
+Require Import Proofs.Var.
+Require Import Proofs.VarSet.
+Require Import Proofs.VarEnv.
+Require Import Unique.Proofs.
+Require Import Proofs.GhcUtils.
+Require Import Proofs.Util.
+
+Set Bullet Behavior "Strict Subproofs".
+
+Close Scope Z_scope.
+
+Definition WellScoped_VarEnv ( venv : VarEnv Var) (vs:VarSet) : Prop :=
+  forall var,  match lookupVarEnv venv var with
+        | Some v' => WellScopedVar v' vs
+        | None => True
+        end.
+
+
+Definition WellScoped_TidyEnv : Core.TidyEnv -> VarSet -> Prop :=
+  fun env vs => match env with 
+             | (oenv, venv) => WellScoped_VarEnv venv vs
+             end.
+  
+
+Lemma coreTidy_wellScoped : forall e env vs,
+    WellScoped_TidyEnv env vs -> 
+    WellScoped e vs -> 
+    WellScoped (tidyExpr env e) vs.
+Proof.
+  intros e.
+  apply (core_induct e); unfold tidyExpr.
+  - move=> v [oenv venv] vs WSenv WSe.
+    simpl. 
+    destruct (lookupVarEnv venv v) eqn:IN; simpl. 
+    simpl in WSenv, WSe. unfold WellScoped_VarEnv in WSenv. specialize (WSenv v). rewrite IN in WSenv. auto. 
+    simpl in WSe. auto.
+  - intros. auto.
+Admitted.
