examples/ghc/theories/StrongFV.v
@@ -1,0 +1,793 @@
+(* Disable notation conflict warnings *)
+Set Warnings "-notation-overridden".
+
+From mathcomp.ssreflect
+Require Import ssreflect ssrnat prime ssrbool eqtype.
+
+Require Import Core.
+Require Import FV.
+Require Import Proofs.Axioms.
+Require Import Proofs.ContainerAxioms.
+Require Import Proofs.VarSet.
+Require Import Proofs.StrongVarSet.
+Require Import Proofs.Var.
+
+Require Import Coq.Lists.List.
+Require Import Coq.Bool.Bool.
+
+Require Import GHC.Base.
+Require Import Proofs.Prelude.
+Import GHC.Base.ManualNotations.
+
+Require Import Coq.Classes.Morphisms.
+
+Set Bullet Behavior "Strict Subproofs".
+
+Lemma fold_is_true : forall b, b = true <-> b.
+Proof. intros. unfold is_true. reflexivity. Qed.
+
+Lemma RespectsAEVar_const_true : RespectsAEVar (const true).
+Proof. move => x1 x2 Eq. reflexivity. Qed.
+Hint Resolve RespectsAEVar_const_true.
+Lemma RespectsAEVar_andb f0 f: 
+  RespectsAEVar f0 -> RespectsAEVar f ->
+  RespectsAEVar (fun v : Var => f0 v && f v).
+Proof.
+  move => r1 r2 x1 x2 Eq.
+  erewrite r1; eauto. 
+  erewrite r2; eauto.
+Qed.
+
+Lemma emptyVarSet_StrongSubset :
+  forall vs, emptyVarSet {<=} vs.
+Admitted.
+Hint Resolve emptyVarSet_StrongSubset.
+
+
+Instance StrongSubset_m : Proper (StrongEquivalence ==> StrongEquivalence ==> iff) StrongSubset.
+Admitted.
+
+(* ---- Extensional Equality for VarSets --- *)
+
+(*
+Definition extEqual vs1 vs2 := forall v, lookupVarSet vs1 v = lookupVarSet vs2 v.
+Definition extSubset vs1 vs2 := forall v v1, lookupVarSet vs1 v = Some v1 -> lookupVarSet vs2 v = Some v1.
+
+Notation "vs1 |=| vs2" := (extEqual vs1 vs2) (at level 70, no associativity).
+Notation "vs1 |<=| vs2" := (extSubset vs1 vs2) (at level 70, no associativity).
+
+Instance extEqual_Reflexive : Reflexive extEqual.
+Proof. move => vs v. auto. Qed.
+Instance extEqual_Symmetric : Symmetric extEqual.
+Proof. move => vs1 vs2 E v. rewrite (E v). done. Qed.
+Instance extEqual_Transitive : Transitive extEqual.
+Proof. move => vs1 vs2 vs3 E1 E2 v. rewrite (E1 v). rewrite (E2 v). done. Qed.
+*)
+
+(* This is actually a fairly strong statement of our VarSet implementation. It says that the VarSets are 'parametric' 
+   WRT to the non-unique information stored in the Var. In other words, 
+   we know that there is no way to produce the following situation (where 123 is the unique, 
+   A/B is the aux info.)
+
+      123_A  ...  `unionVarSet` 123_B  =>  123_A ...
+
+      123_A  ... `unionVarSet`  123_B   =>  123_B ...
+*)
+Instance unionVarSet_m : Proper (StrongEquivalence ==> StrongEquivalence ==> StrongEquivalence) unionVarSet.
+Proof.
+Admitted.
+(*
+  move=> [[x1]] [[y1]] E1 [[x2]] [[y2]] E2.
+  move=> v.
+  move: (E1 v) (E2 v) => e1 e2.
+  unfold lookupVarSet,UniqSet.lookupUniqSet,UniqFM.lookupUFM  in *.
+  set (k := (Unique.getWordKey (Unique.getUnique v))) in *.
+  unfold unionVarSet, UniqSet.unionUniqSets, UniqFM.plusUFM.
+  destruct (IntMap.lookup k x2) eqn:L2; 
+  destruct (IntMap.lookup k x1) eqn:L1.
+  + move: (lookup_union _ k v0 x2 x1) => [hx _].
+    move: (lookup_union _ k v0 y2 y1) => [hy _].
+    rewrite hx. rewrite hy.   
+    done.
+    left. done.
+    left. done.
+  + move: (lookup_union _ k v0 x2 x1) => [hx _].
+    move: (lookup_union _ k v0 y2 y1) => [hy _].
+    rewrite hx. rewrite hy.   
+    done.
+    left. done.
+    left. done.
+  + move: (lookup_union _ k v0 x2 x1) => [hx _].
+    move: (lookup_union _ k v0 y2 y1) => [hy _].
+    rewrite hx. rewrite hy.   
+    done.
+    right. done.
+    right. done.
+  + symmetry in e1. rewrite <- non_member_lookup in e1.
+    symmetry in e2. rewrite <- non_member_lookup in e2.
+    (* seems provable but fussy. *)
+Admitted.  *)
+
+Instance minusVarSet_ext_m : Proper (StrongEquivalence ==> StrongEquivalence ==> StrongEquivalence) minusVarSet.
+Proof.
+  move=> [[x1]] [[y1]] E1 [[x2]] [[y2]] E2.
+(*  move=> v.
+  move: (E1 v) (E2 v) => e1 e2.
+  unfold lookupVarSet,UniqSet.lookupUniqSet,UniqFM.lookupUFM  in *.
+  set (k := (Unique.getWordKey (Unique.getUnique v))) in *.
+  unfold minusVarSet, UniqSet.minusUniqSet, UniqFM.minusUFM.
+  destruct (IntMap.lookup k x2) eqn:L2. symmetry in e2.
+  erewrite lookup_difference_in_snd; eauto.
+  erewrite lookup_difference_in_snd; eauto.
+  rewrite lookup_difference_not_in_snd; eauto.
+  rewrite lookup_difference_not_in_snd; eauto.
+Qed. *)
+Admitted.
+
+Instance filterVarSet_ext_m : 
+  forall f, RespectsAEVar f ->
+  Proper (StrongEquivalence ==> StrongEquivalence) (filterVarSet f).
+Proof.
+(*   move=> v.
+   move: (E2 v) => e2.
+   unfold lookupVarSet,UniqSet.lookupUniqSet,UniqFM.lookupUFM  in *.
+   set (k := (Unique.getWordKey (Unique.getUnique v))) in *.
+   unfold filterVarSet,UniqSet.filterUniqSet,UniqFM.filterUFM. *)
+Admitted.
+
+Definition almostEqual_option (o1 : option Var) (o2: option Var) : Prop :=
+  match o1 , o2 with 
+  | Some v1 , Some v2 => almostEqual v1 v2
+  | None , None => True 
+  | _ , _ => False
+end.
+
+
+Instance lookupVarSet_ext_m : 
+  Proper (StrongEquivalence ==> almostEqual ==> almostEqual_option) lookupVarSet.
+Proof.
+    move=> [[x1]] [[y1]] E1 v1 v2 E2.
+(*    move: (E1 v1) => e.
+    done.
+Qed. *) 
+Admitted.
+
+Instance elemVarSet_ext_m : Proper (almostEqual ==> StrongEquivalence ==> Logic.eq) elemVarSet.
+Proof.
+    move=> v1 v2 E2 [[x1]] [[y1]] E1 .
+(*    move: (E1 v1) => e. *)
+Admitted.
+
+Instance extendVarSet_ext_m : Proper (StrongEquivalence ==> almostEqual ==> StrongEquivalence) extendVarSet.
+Proof.
+Admitted.
+
+Instance extendVarSetList_ext_m : Proper (StrongEquivalence ==> Forall2 almostEqual ==>  StrongEquivalence) extendVarSetList.
+Proof.
+  move=> vs1 vs2 E1 l1 l2 E2.
+(*  subst l1.
+  move: l2 vs1 vs2 E1.
+  induction l2; move=> vs1 vs2 E1.
+  hs_simpl. done.
+  hs_simpl. erewrite IHl2; eauto.
+  rewrite -> E1. done.
+Qed. *) 
+Admitted.
+  
+Instance delVarSet_ext_m  : Proper (StrongEquivalence ==> almostEqual ==> StrongEquivalence) delVarSet.
+Admitted.
+
+(* -------------------------- *)
+
+
+Lemma unionVarSet_emptyVarSet_l : forall vs, unionVarSet emptyVarSet vs {=} vs.
+Proof.
+  move=> [[i]].
+  unfold lookupVarSet,UniqSet.lookupUniqSet,UniqFM.lookupUFM  in *.
+  simpl.
+Admitted.
+
+Axiom unionVarSet_emptyVarSet_r : forall vs, unionVarSet vs emptyVarSet {=} vs.
+
+
+
+Axiom filterSingleton_true : forall f x,
+  RespectsAEVar f -> f x = true -> filterVarSet f (unitVarSet x) {=} unitVarSet x.
+Axiom filterSingleton_false : forall f x,
+  RespectsAEVar f -> f x = false -> filterVarSet f (unitVarSet x) {=} emptyVarSet.
+  
+Lemma filterVarSet_StrongEquivalence : forall (f : Var -> bool) (vs1 vs2 : VarSet),
+   RespectsAEVar f ->
+   vs1 {=} vs2 -> (filterVarSet f vs1) {=} (filterVarSet f vs2).
+Proof.
+  move => f [[i1]] [[i2]] E.
+  unfold lookupVarSet,UniqSet.lookupUniqSet,UniqFM.lookupUFM  in *.
+  unfold filterVarSet,UniqSet.filterUniqSet,UniqFM.filterUFM.
+Admitted.
+
+Hint Resolve filterVarSet_StrongEquivalence.
+
+Axiom filterVarSet_constTrue:
+  forall vs : VarSet, (filterVarSet (const true) vs) {=} vs.
+
+Axiom filterVarSet_StrongSubset : forall (f : Var -> bool) (vs : VarSet),
+   RespectsAEVar f ->
+   (filterVarSet f vs) {=} vs.
+
+Lemma filterVarSet_comp : forall f f' vs,
+    RespectsAEVar f ->
+    RespectsAEVar f' ->
+    filterVarSet f (filterVarSet f' vs) {=} filterVarSet (fun v => f v && f' v) vs.
+Proof.
+   intros. destruct vs, getUniqSet'. simpl.
+Admitted.
+
+Hint Rewrite unionVarSet_emptyVarSet_l  unionVarSet_emptyVarSet_r : hs_simpl.
+
+
+Lemma minusVarSet_unitVarSet_true : forall x s,
+  elemVarSet x s = true -> 
+  minusVarSet (unitVarSet x) s = emptyVarSet.
+Proof.
+  move=> x [[i]] E.
+Admitted.
+
+(* Maybe this can also be true with '=' *)
+Axiom minusVarSet_unitVarSet_false : forall x s,
+  elemVarSet x s = false -> 
+  minusVarSet (unitVarSet x) s {=} unitVarSet x.
+
+(* This is only true on the left *)
+Lemma unionVarSet_unitVarSet_l x : forall vs0 ,
+  elemVarSet x vs0 = true ->
+  unionVarSet (unitVarSet x) vs0 {=} vs0.
+Proof.
+  move=> [[i]] E.
+Admitted.
+(*
+  move=> v.
+  unfold unionVarSet, UniqSet.unionUniqSets, UniqFM.plusUFM.
+  unfold elemVarSet,UniqSet.elementOfUniqSet,UniqFM.elemUFM  in *.
+  unfold lookupVarSet,UniqSet.lookupUniqSet,UniqFM.lookupUFM  in *.
+  simpl.
+  destruct (IntMap.lookup (realUnique v) i) eqn:L.
+  + rewrite <- lookup_union.
+    left. auto.
+  + destruct (v == x) eqn:Ex.
+    ++ rewrite var_eq_realUnique in Ex.
+       admit.
+    ++ admit.
+Admitted. *)
+
+(* Scoped commutation for VarSet union. *)
+Lemma unionVarSet_commute : forall vs0 vs1 sc,
+  vs0 {<=} sc ->
+  vs1 {<=} sc ->
+  unionVarSet vs0 vs1 {=} unionVarSet vs1 vs0.
+Proof.
+Admitted.
+
+
+Lemma filterVarSet_delVarSet_1 f vs v:
+  RespectsAEVar f ->
+  filterVarSet f (delVarSet vs v) {<=} delVarSet (filterVarSet f vs) v.
+Admitted.
+Lemma filterVarSet_delVarSet_2 f vs v:
+  RespectsAEVar f ->
+  delVarSet (filterVarSet f vs) v {<=} filterVarSet f (delVarSet vs v).
+Admitted.
+Lemma filterVarSet_delVarSet f vs v:
+  RespectsAEVar f ->
+  filterVarSet f (delVarSet vs v) {=} delVarSet (filterVarSet f vs) v.
+Proof.
+  intro Hf. split. eapply filterVarSet_delVarSet_1; eauto.
+  eapply filterVarSet_delVarSet_2; eauto.
+Qed.
+
+Lemma minusVarSet_extendVarSet_1 vs1 vs2 v :
+  minusVarSet vs1 (extendVarSet vs2 v) {<=}
+  minusVarSet (delVarSet vs1 v) vs2. 
+Admitted.
+Lemma minusVarSet_extendVarSet_2 vs1 vs2 v :
+  minusVarSet (delVarSet vs1 v) vs2 {<=}
+  minusVarSet vs1 (extendVarSet vs2 v).
+Admitted.
+Lemma minusVarSet_extendVarSet vs1 vs2 v :
+  minusVarSet vs1 (extendVarSet vs2 v) {=}
+  minusVarSet (delVarSet vs1 v) vs2. 
+Admitted.
+
+
+Axiom unionVarSet_assoc_StrongEquivalence : forall vs1 vs2 vs3,
+  unionVarSet vs1 (unionVarSet vs2 vs3) {=}
+  unionVarSet (unionVarSet vs1 vs2) vs3.
+Axiom unionVarSet_minusVarSet : forall vs1 vs2 vs : VarSet,
+  (unionVarSet (minusVarSet vs1 vs) (minusVarSet vs2 vs)) 
+    {=} (minusVarSet (unionVarSet vs1 vs2) vs).
+Axiom unionVarSet_filterVarSet : forall (f : Var -> bool) (vs1 vs2 : VarSet),
+   RespectsAEVar f ->
+   (unionVarSet (filterVarSet f vs1) (filterVarSet f vs2))
+    {=} (filterVarSet f (unionVarSet vs1 vs2)).
+
+
+(* ------- Denote --------- *)
+
+(* Add the elements in the list in the reverse order *)
+Definition extendVarSetList' vs (l : list Var) :=
+  Foldable.foldr (fun vs0 x => extendVarSet x vs0) vs l.
+
+Lemma extendVarSetList_rev vs l : 
+  extendVarSetList' vs (rev l) = extendVarSetList vs l.
+Proof.
+  unfold extendVarSetList'. rewrite extendVarSetList_foldl'. unfold VarSetFSet.VarSetFSet.add.
+  rewrite hs_coq_foldr_list.
+  rewrite hs_coq_foldl'_list.
+  rewrite fold_left_rev_right.
+  done.
+Qed.
+
+Instance extendVarSetList'_ext_m : Proper (StrongEquivalence ==> Forall2 almostEqual ==>  StrongEquivalence) extendVarSetList'.
+Proof.
+  move=> vs1 vs2 E1 l1 l2 E2.
+(*  subst l1.
+  unfold extendVarSetList'.
+  induction l2. 
+  hs_simpl. done.
+  hs_simpl. 
+  admit. *)
+Admitted.
+
+
+(*
+Lemma ext_weak vs1 vs2 : vs1 {=} vs2 -> vs1 [=] vs2.
+Proof.
+  move=> h v .
+  move: (h v) => hv.
+  unfold VarSetFSet.In.
+  split; move=> h1.
+  all: apply elemVarSet_lookupVarSet in h1.
+  all: move: h1 => [var h2].
+  rewrite -> hv in h2. eapply lookupVarSet_elemVarSet; eauto.
+  rewrite <- hv in h2. eapply lookupVarSet_elemVarSet; eauto.
+Qed.
+*)
+
+
+
+(* NOTE: 
+
+      The lists are the "real" representation of the set and are stored in reverse order.
+      The sets (vs0 and vs1) are only used for expedient equality testing.
+
+      NO: this is not true. fvVarSet 
+
+      FV = InterestingVarFun -> VarSet -> list Var * VarSet -> list Var * VarSet
+*)
+
+Inductive Denotes : VarSet -> FV -> VarSet -> Prop :=
+| DenotesVarSet : forall vs fv out_scope,
+    (forall f in_scope l0 vs0,
+        RespectsAEVar f ->
+        vs0 {<=} out_scope ->
+        let vl0        := extendVarSetList' emptyVarSet l0 in
+        vl0 {=} vs0 ->
+        let '(l1, vs1) := fv f in_scope (l0, vs0) in
+        let vl1        := extendVarSetList' emptyVarSet l1 in
+        vl1 {=} vs1 /\
+        vs1 {=} unionVarSet vs0 (minusVarSet (filterVarSet f vs) in_scope) /\
+        vs1 {<=} out_scope) ->
+    Denotes vs fv out_scope.
+Notation "A ⊢ B <={ C } " := (Denotes A B C) (at level 70).
+
+
+Theorem Denotes_fvVarSet : forall m fv sc f in_scope l0 vs0,
+    (m ⊢ fv <={ sc }) ->
+    RespectsAEVar f ->
+    extendVarSetList' emptyVarSet l0 {=} vs0 ->
+    vs0 {<=} sc ->
+    snd (fv f in_scope (l0, vs0))
+      {=} unionVarSet vs0 (minusVarSet (filterVarSet f m) in_scope) /\
+    snd (fv f in_scope (l0, vs0)) 
+      {<=} sc.
+Proof.
+  move => m fv sc f in_scope l0 vs0 [vs' fv' out H0] H1 H2 H3.
+  specialize (H0 f in_scope l0 vs0 H1 H3); subst.
+  set (vl0 := extendVarSetList' emptyVarSet l0) in *.
+  destruct fv'.
+  specialize (H0 H2).
+  set (vl1 := extendVarSetList' emptyVarSet l) in *.
+  simpl in H0.
+  move: H0 => [h0 [h1 h2]].
+  simpl.
+  done.
+Qed.
+
+
+
+Instance Denotes_m : 
+  Proper (StrongEquivalence ==> Logic.eq ==> StrongEquivalence ==> iff) Denotes.
+Admitted.
+
+Lemma Denotes_weaken vs fv sc1 sc2:
+  sc1 {<=} sc2 -> Denotes vs fv sc1 -> Denotes vs fv sc2.
+Proof.  
+Admitted.
+
+Definition WF_fv (fv : FV) sc : Prop := exists vs, Denotes vs fv sc.
+
+(* -------------------------------------------- *)
+
+Lemma emptyVarSet_emptyFV sc : Denotes emptyVarSet emptyFV sc.
+Proof.
+  constructor; intros; subst.
+  unfold emptyFV.
+  split; auto.
+  hs_simpl.
+  split; eauto.
+  reflexivity.
+Qed.
+
+
+Lemma empty_FV_WF sc :
+  WF_fv emptyFV sc.
+Proof.
+  unfold WF_fv. exists emptyVarSet. eapply emptyVarSet_emptyFV. 
+Qed.
+
+
+Lemma unitVarSet_unitFV x sc : 
+   unitVarSet x {<=} sc ->
+   Denotes (unitVarSet x) (unitFV x) sc.
+Proof.
+  constructor; intros; subst.
+  unfold unitFV.
+  destruct elemVarSet eqn:E1;
+  destruct (f x) eqn:FX;
+  hs_simpl. 
+  all: try (split; auto).
+  - rewrite -> filterSingleton_true; try done.
+    rewrite -> minusVarSet_unitVarSet_true; try done.
+    hs_simpl. 
+    split. reflexivity. done.
+  - rewrite -> filterSingleton_false; try done.
+    hs_simpl. 
+    split. reflexivity. done.
+  - elim In: (elemVarSet x vs0) => //.  split; auto.
+    + rewrite -> filterSingleton_true => //.
+      rewrite -> minusVarSet_unitVarSet_false; try done.  
+      rewrite unionVarSet_commute; eauto.
+      rewrite -> unionVarSet_unitVarSet_l; eauto. 
+      split. reflexivity. done.
+    + unfold extendVarSetList' .
+      hs_simpl.
+      split.
+      f_equiv. auto.
+      split.
+      rewrite -> filterSingleton_true => //.      
+      rewrite -> minusVarSet_unitVarSet_false => //.
+      ++ admit.
+      ++ admit.
+Admitted.
+
+Lemma unit_FV_WF x sc :
+  unitVarSet x {<=} sc ->
+  WF_fv (unitFV x) sc.
+Proof.
+   unfold WF_fv.
+  exists (unitVarSet x).
+  eapply unitVarSet_unitFV; eauto.
+Qed.
+
+
+Lemma filterVarSet_filterFV f vs x sc:
+  RespectsAEVar f ->
+  Denotes vs x sc -> Denotes (filterVarSet f vs) (filterFV f x) sc.
+Proof.
+  move => p D.
+  constructor. move=> f0 in_scope vs' l h0 h1 l1 h2.
+  inversion D.
+  unfold filterFV. subst.
+
+  specialize (H (fun v : Var => f0 v && f v) in_scope vs' l 
+                ltac:(eauto using RespectsAEVar_andb)
+                ltac:(auto)
+                ltac:(eauto)
+               ).
+  destruct x.
+  set (vl1:= extendVarSetList' emptyVarSet l0) in *.
+  destruct H as [k0 [k1 k2]].
+  split; auto. split; auto.
+  rewrite <- filterVarSet_comp in k1; eauto.
+Qed.
+
+Ltac unfold_WF :=
+  repeat match goal with
+  | [ H : WF_fv ?fv ?sc |- _] =>
+    let vs := fresh "vs" in
+    let Hd := fresh "Hdenotes" in
+    inversion H as [vs Hd]; inversion Hd; subst; clear H
+  | [ |- WF_fv ?fv ?sc] =>
+    unfold WF_fv
+  end.
+
+Lemma filter_FV_WF : forall f x sc,
+    RespectsAEVar f ->
+    WF_fv x sc -> WF_fv (filterFV f x) sc.
+Proof.
+  intros. unfold_WF.
+  exists (filterVarSet f vs). 
+  eapply filterVarSet_filterFV; auto.
+Qed.
+
+Axiom delVarSet_StrongSubset : forall xs v sc,
+  xs {<=} sc ->
+  delVarSet xs v {<=} sc.
+
+
+Lemma delVarSet_delFV vs v fv sc :
+  Denotes vs fv sc -> Denotes (delVarSet vs v) (delFV v fv) (delVarSet sc v).
+Proof.
+  move=> H. inversion H. subst.
+  constructor; intros. unfold delFV.
+  specialize (H0 f (extendVarSet in_scope v) l0 vs0 H1).
+  have h0: vs0 {<=} sc. { eapply StrongSubset_trans; eauto.
+                         eapply delVarSet_StrongSubset; eauto. reflexivity.
+                       }
+  specialize (H0 h0 H3).
+  destruct fv.
+  set (vl1 := extendVarSetList' emptyVarSet l) in *. 
+  destruct H0 as [h1 [h2 h3]].
+  split; auto.
+  split.
+  rewrite -> h2. 
+  f_equiv.
+  rewrite filterVarSet_delVarSet; eauto.
+  rewrite minusVarSet_extendVarSet; eauto.
+  reflexivity.
+  (* Ugh. need to argue that v is not in v0 *)
+  (* we know this because v is not in vs0 
+     and it is subtracted out from filterVarSet f vs *)
+  admit.
+Admitted.
+
+
+Lemma del_FV_WF : forall fv v sc,
+    WF_fv fv sc -> WF_fv (delFV v fv) (delVarSet sc v).
+Proof.
+  intros. unfold_WF.
+  exists (delVarSet vs v). 
+  eapply delVarSet_delFV. auto.
+Qed.
+
+Lemma unionVarSet_unionFV vs vs' fv fv' sc:
+  Denotes vs fv sc -> Denotes vs' fv' sc -> Denotes (unionVarSet vs vs') (unionFV fv' fv) sc.
+Proof.
+  move=> H H1. inversion H. inversion H1. subst.
+  constructor.
+  move=> f in_scope l0 vs0 h h0.
+  move=> vl0 h1.
+  unfold unionFV.
+  specialize (H0 f in_scope l0 vs0 h h0 h1).  
+  set (vs_mid := (fv f in_scope (l0, vs0))) in *. destruct vs_mid as [l1 vs1].
+  move: H0 => [h2 [h3 h4]].
+  specialize (H5 f in_scope l1 vs1 ltac:(auto) ltac:(auto) ltac:(eauto)).  
+  destruct fv' as [l2 vs2].
+  move: H5 => [h5 [h6 h7]].
+  split. auto.
+  split; auto. 
+  rewrite -> h6.
+  rewrite -> h3.
+
+  rewrite <- unionVarSet_assoc_StrongEquivalence.
+  f_equiv.
+  rewrite -> unionVarSet_minusVarSet.  
+  f_equiv.
+  rewrite unionVarSet_filterVarSet => //.
+  reflexivity. 
+Qed.
+
+Lemma union_FV_WF : forall fv fv' vs,
+    WF_fv fv vs -> WF_fv fv' vs -> WF_fv (unionFV fv fv') vs.
+Proof.
+  intros. unfold_WF.
+  exists (unionVarSet vs0 vs1). 
+  eapply unionVarSet_unionFV; eauto.
+Qed.  
+
+
+Lemma mapUnionFV_nil A f : 
+  mapUnionFV f (nil : list A) = emptyFV.
+Proof.
+  simpl.
+  unfold emptyFV.
+  reflexivity.
+Qed. 
+Hint Rewrite mapUnionFV_nil : hs_simpl. 
+
+Lemma mapUnionFV_cons A f (x : A) xs : 
+  mapUnionFV f (x :: xs) = unionFV (mapUnionFV f xs) (f x).
+Proof.
+  simpl.
+  unfold unionFV.
+  reflexivity.
+Qed.
+Hint Rewrite mapUnionFV_cons : hs_simpl. 
+
+
+Lemma map_union_FV_WF : forall A f vs (ls : list A),
+    (forall e, In e ls -> WF_fv (f e) vs) ->
+    WF_fv (mapUnionFV f ls) vs.
+Proof.
+  induction ls.
+  - intros.
+    exists emptyVarSet.
+    hs_simpl.
+    eapply emptyVarSet_emptyFV.
+  -  move=> h. simpl in h.
+    assert (h0 : forall e : A, In e ls -> WF_fv (f e) vs). { intros. apply h. tauto. }
+    apply IHls in h0.
+    assert (WF_fv (f a) vs). { apply h; tauto. }
+    hs_simpl.
+    move: h0 => [vs1 D1].
+    move: H => [vs' D'].
+    eexists.
+    eapply unionVarSet_unionFV; eauto.
+Qed.
+
+Lemma unions_FV_WF : forall fvs vs,
+    (forall fv, In fv fvs -> WF_fv fv vs) ->
+    WF_fv (unionsFV fvs) vs.
+Proof.
+  intros.
+  eapply map_union_FV_WF. auto.
+Qed.
+
+
+Lemma mkFVs_FV_WF : forall vs sc,
+    (forall v, In v vs -> unitVarSet v {<=} sc) ->
+    WF_fv (mkFVs vs) sc.
+Proof.
+  intros. apply map_union_FV_WF; intros. apply unit_FV_WF.
+  eauto.
+Qed.
+
+Hint Resolve unit_FV_WF.
+Hint Resolve empty_FV_WF.
+Hint Resolve union_FV_WF.
+Hint Resolve unions_FV_WF.
+Hint Resolve del_FV_WF.
+Hint Resolve mkFVs_FV_WF.
+
+(** * Some other theroems about [FV]s. *)
+
+
+Lemma union_empty_l : forall fv, FV.unionFV FV.emptyFV fv = fv.
+Proof. reflexivity. Qed.
+
+Lemma union_empty_r : forall fv, FV.unionFV fv FV.emptyFV = fv.
+Proof. reflexivity. Qed.
+
+
+Lemma Denotes_fvVarSet_vs vs fv sc :
+  Denotes vs fv sc -> fvVarSet fv {=} vs.
+Proof.
+  move => [vs0 fv0 sc0 h1].
+  unfold fvVarSet, op_z2218U__, fvVarListVarSet.
+  specialize (h1 (const true) emptyVarSet nil emptyVarSet ltac:(eauto) 
+    ltac:(eauto)).
+  unfold extendVarSetList' in h1. hs_simpl in h1.
+  destruct fv0 as [l1 vs1].
+  destruct h1 as [h2 [h3 h4]]. reflexivity.
+  simpl.
+  rewrite -> h3.
+  rewrite unionVarSet_emptyVarSet_l.
+  rewrite filterVarSet_constTrue.
+  reflexivity.
+Qed.
+
+Lemma Denotes_sc vs fv sc :
+  Denotes vs fv sc -> vs {<=} sc.
+Proof.
+  move=> [vs0 fv0 sc0 h1].
+  unfold fvVarSet, op_z2218U__, fvVarListVarSet.
+  specialize (h1 (const true) emptyVarSet nil emptyVarSet ltac:(eauto) 
+    ltac:(eauto)).
+  unfold extendVarSetList' in h1. hs_simpl in h1.
+  destruct fv0 as [l1 vs1].
+  destruct h1 as [h2 [h3 h4]]. reflexivity.
+  hs_simpl in h3.
+  rewrite -> filterVarSet_constTrue in h3.
+  rewrite <- h3.
+  auto.
+Qed.
+
+
+Lemma Denotes_inj1 vs1 vs2 fv sc : Denotes vs1 fv sc -> Denotes vs2 fv sc -> vs1 {=} vs2.
+Proof.      
+  move => h1. inversion h1.
+  move => h2. inversion h2.
+  subst.
+  set in_scope := emptyVarSet.
+  assert (h : extendVarSetList emptyVarSet nil {=} emptyVarSet).
+  { rewrite <- mkVarSet_extendVarSetList. reflexivity. }
+  specialize (H (const true) in_scope nil emptyVarSet ltac:(auto) ltac:(auto) h).
+  specialize (H3 (const true) in_scope nil emptyVarSet ltac:(auto) ltac:(auto) h).
+  destruct fv as [l3 vs3].
+  move: H => [h3 [h4 hg]].
+  move: H3 => [h5 [h6 hh]].
+  hs_simpl in h4.
+  hs_simpl in h6.
+  rewrite -> filterVarSet_constTrue in h4.
+  rewrite -> filterVarSet_constTrue in h6.
+  rewrite <- h4.
+  rewrite <- h6.
+  reflexivity.
+Qed.
+
+
+Lemma delVarSet_fvVarSet: forall fv x sc,
+    WF_fv fv sc ->
+    delVarSet (fvVarSet fv) x {=} fvVarSet (delFV x fv).
+Proof.
+  move => fv x sc [vs D].
+  move: (delVarSet_delFV _ x _ sc D) => h1.
+  move: (Denotes_fvVarSet_vs _ _ _ h1) => h2.
+  move: (Denotes_fvVarSet_vs _ _ _ D) => h3.
+  rewrite h2.
+  rewrite h3.
+  reflexivity.
+Qed.
+
+Lemma mapUnionVarSet_mapUnionFV A (ps : list A) 
+      (f1 :  A -> VarSet) (f2 : A -> FV.FV) sc :
+  Forall2 (fun vs fv => Denotes vs fv sc) (map f1 ps) (map f2 ps) ->
+  Denotes  (mapUnionVarSet f1 ps) (FV.mapUnionFV f2 ps) sc.
+Proof.
+  elim: ps => [|p ps IH]; unfold mapUnionVarSet; simpl.
+  hs_simpl.
+  - move=>h. constructor; intros; subst.
+    hs_simpl.
+    split; auto.
+    split.
+    reflexivity.
+    auto.
+  - hs_simpl.
+    move=>h. inversion h. subst.
+    unfold mapUnionVarSet in IH.
+    specialize (IH H4). clear H4.
+    move: (unionVarSet_unionFV _ _ _ _ _ H2 IH) => h0.
+    unfold FV.unionFV in h0.
+    auto.
+Qed.
+
+
+Lemma unionsFV_cons fv fvs : 
+  FV.unionsFV (fv :: fvs) = 
+  FV.unionFV (FV.unionsFV fvs) fv.
+Proof.
+  repeat unfold FV.unionsFV, FV.unionFV.
+  rewrite mapUnionFV_cons.
+  unfold FV.unionFV.
+  simpl.
+  reflexivity.
+Qed.
+
+
+Lemma unionsVarSet_unionsFV vss fvs sc: 
+   Forall2 (fun vs fv => Denotes vs fv sc) vss fvs ->
+   Denotes (Foldable.foldr unionVarSet emptyVarSet vss) (FV.unionsFV fvs) sc.
+Proof.
+  elim.
+  - hs_simpl. 
+    unfold FV.unionsFV, FV.mapUnionFV.
+    constructor; intros; subst.
+    hs_simpl.
+    split; auto.
+    split; auto. reflexivity.
+  - move => vs fv vss1 fvs1 D1 D2 IH. 
+    hs_simpl. 
+    move: (unionVarSet_unionFV _ _ _ _ _ D1 IH) => h0.
+    rewrite unionsFV_cons.
+    auto.
+Qed.
+
